lean/Eyg.lean
@@ -28,8 +28,5 @@ import Eyg.Types.Runtime
 import Eyg.Types.Machine
 import Eyg.Types.Substitution
 import Eyg.Types.Generalization
-import Eyg.Types.TypingAt
-import Eyg.Types.TypingAtV
-import Eyg.Types.RuntimeAtV
 import Eyg.Types.CexEffectfulFix
 import Eyg.Types.LevelTagSpike
